formal/nightstream-lean/Nightstream/Rv64IM/Generated/Cases/Case_aligned_negative_offset_roundtrip/Derived.lean
@@ -8,11 +8,15 @@ def derivedCase : ParityDerivedCase :=
   {
   manifest := { name := "aligned_negative_offset_roundtrip", fixtureId := "aligned_negative_offset_roundtrip_v1", protocolVersionId := 1, loweringVersionId := 1, familyTags := [.nativeAlu, .alignedMemory, .controlFlow] }
   , executionRows := [{
-  stepIndex := 0
+  traceIndex := 0
+  , stepIndex := 0
+  , sequenceIndex := 0
   , pc := 0
   , nextPc := 4
   , word := 44040339
   , opcode := .addi
+  , traceOpcode := (some .addi)
+  , traceVirtualOpcode := none
   , family := .nativeAlu
   , rs1 := 0
   , rs1Value := 0
@@ -29,12 +33,21 @@ def derivedCase : ParityDerivedCase :=
   , writesRd := true
   , writesRam := false
   , halted := false
+  , isFirstInSequence := true
+  , virtualSequenceRemaining := none
+  , isEffectRow := true
+  , isCommitRow := true
+  , isReal := true
 }, {
-  stepIndex := 1
+  traceIndex := 1
+  , stepIndex := 1
+  , sequenceIndex := 0
   , pc := 4
   , nextPc := 8
   , word := 4262804515
   , opcode := .sd
+  , traceOpcode := (some .sd)
+  , traceVirtualOpcode := none
   , family := .alignedMemory
   , rs1 := 10
   , rs1Value := 8200
@@ -51,12 +64,21 @@ def derivedCase : ParityDerivedCase :=
   , writesRd := false
   , writesRam := true
   , halted := false
+  , isFirstInSequence := true
+  , virtualSequenceRemaining := none
+  , isEffectRow := true
+  , isCommitRow := true
+  , isReal := true
 }, {
-  stepIndex := 2
+  traceIndex := 2
+  , stepIndex := 2
+  , sequenceIndex := 0
   , pc := 8
   , nextPc := 12
   , word := 4286918915
   , opcode := .ld
+  , traceOpcode := (some .ld)
+  , traceVirtualOpcode := none
   , family := .alignedMemory
   , rs1 := 10
   , rs1Value := 8200
@@ -73,12 +95,21 @@ def derivedCase : ParityDerivedCase :=
   , writesRd := true
   , writesRam := false
   , halted := false
+  , isFirstInSequence := true
+  , virtualSequenceRemaining := none
+  , isEffectRow := true
+  , isCommitRow := true
+  , isReal := true
 }, {
-  stepIndex := 3
+  traceIndex := 3
+  , stepIndex := 3
+  , sequenceIndex := 0
   , pc := 12
   , nextPc := 16
   , word := 115
   , opcode := .ecall
+  , traceOpcode := (some .ecall)
+  , traceVirtualOpcode := none
   , family := .controlFlow
   , rs1 := 0
   , rs1Value := 0
@@ -95,13 +126,18 @@ def derivedCase : ParityDerivedCase :=
   , writesRd := false
   , writesRam := false
   , halted := true
+  , isFirstInSequence := true
+  , virtualSequenceRemaining := none
+  , isEffectRow := true
+  , isCommitRow := true
+  , isReal := true
 }]
-  , stage1 := { rows := [{ stepIndex := 0, fetchPc := 0, fetchedWord := 44040339, opcode := .addi, family := .nativeAlu, nextPc := 4, aluResult := 42, effectiveAddr := none, writesRd := true, rd := 1, rdAfter := 42, preservesX0 := false }, { stepIndex := 1, fetchPc := 4, fetchedWord := 4262804515, opcode := .sd, family := .alignedMemory, nextPc := 8, aluResult := 42, effectiveAddr := (some 8192), writesRd := false, rd := 0, rdAfter := 0, preservesX0 := true }, { stepIndex := 2, fetchPc := 8, fetchedWord := 4286918915, opcode := .ld, family := .alignedMemory, nextPc := 12, aluResult := 42, effectiveAddr := (some 8192), writesRd := true, rd := 2, rdAfter := 42, preservesX0 := false }, { stepIndex := 3, fetchPc := 12, fetchedWord := 115, opcode := .ecall, family := .controlFlow, nextPc := 16, aluResult := 0, effectiveAddr := none, writesRd := false, rd := 0, rdAfter := 0, preservesX0 := true }] }
+  , stage1 := { rows := [{ traceIndex := 0, stepIndex := 0, sequenceIndex := 0, fetchPc := 0, fetchedWord := 44040339, opcode := .addi, traceOpcode := (some .addi), traceVirtualOpcode := none, family := .nativeAlu, nextPc := 4, aluResult := 42, effectiveAddr := none, writesRd := true, rd := 1, rdAfter := 42, isFirstInSequence := true, virtualSequenceRemaining := none, isEffectRow := true, isCommitRow := true, isReal := true, preservesX0 := false }, { traceIndex := 1, stepIndex := 1, sequenceIndex := 0, fetchPc := 4, fetchedWord := 4262804515, opcode := .sd, traceOpcode := (some .sd), traceVirtualOpcode := none, family := .alignedMemory, nextPc := 8, aluResult := 42, effectiveAddr := (some 8192), writesRd := false, rd := 0, rdAfter := 0, isFirstInSequence := true, virtualSequenceRemaining := none, isEffectRow := true, isCommitRow := true, isReal := true, preservesX0 := true }, { traceIndex := 2, stepIndex := 2, sequenceIndex := 0, fetchPc := 8, fetchedWord := 4286918915, opcode := .ld, traceOpcode := (some .ld), traceVirtualOpcode := none, family := .alignedMemory, nextPc := 12, aluResult := 42, effectiveAddr := (some 8192), writesRd := true, rd := 2, rdAfter := 42, isFirstInSequence := true, virtualSequenceRemaining := none, isEffectRow := true, isCommitRow := true, isReal := true, preservesX0 := false }, { traceIndex := 3, stepIndex := 3, sequenceIndex := 0, fetchPc := 12, fetchedWord := 115, opcode := .ecall, traceOpcode := (some .ecall), traceVirtualOpcode := none, family := .controlFlow, nextPc := 16, aluResult := 0, effectiveAddr := none, writesRd := false, rd := 0, rdAfter := 0, isFirstInSequence := true, virtualSequenceRemaining := none, isEffectRow := true, isCommitRow := true, isReal := true, preservesX0 := true }] }
   , stage2 := {
-  registerReads := [{ stepIndex := 0, role := .rs1, reg := 0, value := 0 }, { stepIndex := 1, role := .rs1, reg := 10, value := 8200 }, { stepIndex := 2, role := .rs1, reg := 10, value := 8200 }]
-  , registerWrites := [{ stepIndex := 0, reg := 1, previous := 0, next := 42 }, { stepIndex := 2, reg := 2, previous := 0, next := 42 }]
-  , ramEvents := [{ stepIndex := 1, kind := .write, addr := 8192, previous := 13, next := 42 }, { stepIndex := 2, kind := .read, addr := 8192, previous := 42, next := 42 }]
-  , twistLinks := [{ stepIndex := 0, family := .nativeAlu, routedWriteValue := (some 42), routedMemoryBefore := none, routedMemoryAfter := none }, { stepIndex := 1, family := .alignedMemory, routedWriteValue := none, routedMemoryBefore := (some 13), routedMemoryAfter := (some 42) }, { stepIndex := 2, family := .alignedMemory, routedWriteValue := (some 42), routedMemoryBefore := (some 42), routedMemoryAfter := (some 42) }, { stepIndex := 3, family := .controlFlow, routedWriteValue := none, routedMemoryBefore := none, routedMemoryAfter := none }]
+  registerReads := [{ traceIndex := 0, stepIndex := 0, role := .rs1, reg := 0, value := 0 }, { traceIndex := 1, stepIndex := 1, role := .rs1, reg := 10, value := 8200 }, { traceIndex := 1, stepIndex := 1, role := .rs2, reg := 1, value := 42 }, { traceIndex := 2, stepIndex := 2, role := .rs1, reg := 10, value := 8200 }]
+  , registerWrites := [{ traceIndex := 0, stepIndex := 0, reg := 1, previous := 0, next := 42 }, { traceIndex := 2, stepIndex := 2, reg := 2, previous := 0, next := 42 }]
+  , ramEvents := [{ traceIndex := 1, stepIndex := 1, kind := .write, addr := 8192, previous := 13, next := 42 }, { traceIndex := 2, stepIndex := 2, kind := .read, addr := 8192, previous := 42, next := 42 }]
+  , twistLinks := [{ traceIndex := 0, stepIndex := 0, family := .nativeAlu, routedWriteValue := (some 42), routedMemoryBefore := none, routedMemoryAfter := none }, { traceIndex := 1, stepIndex := 1, family := .alignedMemory, routedWriteValue := none, routedMemoryBefore := (some 13), routedMemoryAfter := (some 42) }, { traceIndex := 2, stepIndex := 2, family := .alignedMemory, routedWriteValue := (some 42), routedMemoryBefore := (some 42), routedMemoryAfter := (some 42) }, { traceIndex := 3, stepIndex := 3, family := .controlFlow, routedWriteValue := none, routedMemoryBefore := none, routedMemoryAfter := none }]
 }
   , stage3 := {
   continuity := [{ stepIndex := 0, pc := 0, nextPc := 4, successorPc := (some 4), finalStep := false, continuityHolds := true }, { stepIndex := 1, pc := 4, nextPc := 8, successorPc := (some 8), finalStep := false, continuityHolds := true }, { stepIndex := 2, pc := 8, nextPc := 12, successorPc := (some 12), finalStep := false, continuityHolds := true }, { stepIndex := 3, pc := 12, nextPc := 16, successorPc := none, finalStep := true, continuityHolds := true }]
@@ -175,10 +211,10 @@ def derivedCase : ParityDerivedCase :=
 }, {
   kind := .appendMessage
   , label := (bytes [114, 118, 54, 52, 105, 109, 47, 107, 101, 114, 110, 101, 108, 47, 115, 116, 97, 103, 101, 49, 95, 100, 105, 103, 101, 115, 116])
-  , message := (bytes [133, 33, 172, 140, 233, 72, 46, 209, 48, 165, 182, 74, 209, 48, 22, 152, 88, 9, 98, 197, 159, 186, 241, 163, 39, 42, 69, 121, 8, 165, 34, 71])
+  , message := (bytes [142, 217, 182, 138, 150, 76, 176, 209, 117, 25, 246, 139, 222, 66, 241, 101, 236, 89, 218, 142, 67, 238, 206, 4, 53, 48, 117, 115, 130, 138, 60, 69])
   , u64s := []
   , cursorBefore := { stateWords := [1056787187556541480, 7936538220362538745, 12726305489166155438, 10033257191059226404, 13102544229850939383, 12364778379655857612, 15189509943256782053, 10541895786105299061], absorbed := 0 }
-  , cursorAfter := { stateWords := [44971546151262230, 34134519537988026, 1193452808, 17884890454721098756, 8742815067097544182, 5833030316974842334, 14069376335563075677, 3519699764892988818], absorbed := 3 }
+  , cursorAfter := { stateWords := [19015891902293489, 32498472230113006, 1161595522, 5217794296179387164, 7843225697845465923, 11072686435381559239, 2494925774217267229, 11700978844590771639], absorbed := 3 }
   , challengeOutput := none
   , digestOutput := none
 }, {
@@ -186,26 +222,26 @@ def derivedCase : ParityDerivedCase :=
   , label := (bytes [114, 118, 54, 52, 105, 109, 47, 115, 116, 97, 103, 101, 50, 47, 114, 101, 103, 95, 109, 105, 120])
   , message := (bytes [])
   , u64s := []
-  , cursorBefore := { stateWords := [44971546151262230, 34134519537988026, 1193452808, 17884890454721098756, 8742815067097544182, 5833030316974842334, 14069376335563075677, 3519699764892988818], absorbed := 3 }
-  , cursorAfter := { stateWords := [4238065095073052119, 7684052836494449271, 7854541950336389888, 7221685285076890941, 14401953932402353816, 15749992700437426292, 2494728818235671694, 1880941987735485193], absorbed := 0 }
-  , challengeOutput := (some 4238065095073052119)
+  , cursorBefore := { stateWords := [19015891902293489, 32498472230113006, 1161595522, 5217794296179387164, 7843225697845465923, 11072686435381559239, 2494925774217267229, 11700978844590771639], absorbed := 3 }
+  , cursorAfter := { stateWords := [9619277481828672587, 665278778681307978, 15723919770595900632, 14028528519789234328, 16076129764726026145, 14784995131326301132, 18180545218882549343, 1705424844785533457], absorbed := 0 }
+  , challengeOutput := (some 9619277481828672587)
   , digestOutput := none
 }, {
   kind := .challengeField
   , label := (bytes [114, 118, 54, 52, 105, 109, 47, 115, 116, 97, 103, 101, 50, 47, 114, 97, 109, 95, 109, 105, 120])
   , message := (bytes [])
   , u64s := []
-  , cursorBefore := { stateWords := [4238065095073052119, 7684052836494449271, 7854541950336389888, 7221685285076890941, 14401953932402353816, 15749992700437426292, 2494728818235671694, 1880941987735485193], absorbed := 0 }
-  , cursorAfter := { stateWords := [14880338601956528058, 11417287982766265704, 1999846905328034605, 3268762540683447153, 3041808325429348029, 11723622584960079147, 3267801232616282909, 1903437023102932086], absorbed := 0 }
-  , challengeOutput := (some 14880338601956528058)
+  , cursorBefore := { stateWords := [9619277481828672587, 665278778681307978, 15723919770595900632, 14028528519789234328, 16076129764726026145, 14784995131326301132, 18180545218882549343, 1705424844785533457], absorbed := 0 }
+  , cursorAfter := { stateWords := [16812727767669355212, 12697392065646144401, 3369600737815196512, 995947170979125272, 9900984208576011045, 13928646283612232713, 2445152170369013135, 1514863595043610672], absorbed := 0 }
+  , challengeOutput := (some 16812727767669355212)
   , digestOutput := none
 }, {
   kind := .appendMessage
   , label := (bytes [114, 118, 54, 52, 105, 109, 47, 107, 101, 114, 110, 101, 108, 47, 115, 116, 97, 103, 101, 50, 95, 100, 105, 103, 101, 115, 116])
-  , message := (bytes [99, 28, 72, 198, 124, 237, 213, 46, 85, 239, 4, 76, 205, 104, 112, 135, 151, 48, 199, 18, 8, 29, 82, 0, 29, 46, 209, 175, 11, 65, 240, 59])
+  , message := (bytes [227, 21, 223, 164, 30, 253, 30, 252, 35, 185, 19, 78, 208, 4, 88, 134, 20, 175, 97, 180, 193, 112, 119, 234, 96, 78, 211, 206, 96, 42, 169, 244])
   , u64s := []
-  , cursorBefore := { stateWords := [14880338601956528058, 11417287982766265704, 1999846905328034605, 3268762540683447153, 3041808325429348029, 11723622584960079147, 3267801232616282909, 1903437023102932086], absorbed := 0 }
-  , cursorAfter := { stateWords := [2272446536714096, 49488116909625885, 1005601035, 16834913648610405511, 10676089165022083198, 2351153205109985000, 15294516587064208466, 12458758220113967936], absorbed := 3 }
+  , cursorBefore := { stateWords := [16812727767669355212, 12697392065646144401, 3369600737815196512, 995947170979125272, 9900984208576011045, 13928646283612232713, 2445152170369013135, 1514863595043610672], absorbed := 0 }
+  , cursorAfter := { stateWords := [54523002147341912, 58216178789283696, 4104727136, 10127024330343439705, 13517581673824157262, 427902716102401987, 3414426687606941972, 18161196869091297655], absorbed := 3 }
   , challengeOutput := none
   , digestOutput := none
 }, {
@@ -213,26 +249,26 @@ def derivedCase : ParityDerivedCase :=
   , label := (bytes [114, 118, 54, 52, 105, 109, 47, 115, 116, 97, 103, 101, 51, 47, 99, 111, 110, 116, 105, 110, 117, 105, 116, 121, 95, 109, 105, 120])
   , message := (bytes [])
   , u64s := []
-  , cursorBefore := { stateWords := [2272446536714096, 49488116909625885, 1005601035, 16834913648610405511, 10676089165022083198, 2351153205109985000, 15294516587064208466, 12458758220113967936], absorbed := 3 }
-  , cursorAfter := { stateWords := [18307016013854385768, 386090934767535184, 301195876403596823, 8691723873807917873, 16010316393357224490, 5609107225314861888, 2143909010010563256, 617300435659316442], absorbed := 0 }
-  , challengeOutput := (some 18307016013854385768)
+  , cursorBefore := { stateWords := [54523002147341912, 58216178789283696, 4104727136, 10127024330343439705, 13517581673824157262, 427902716102401987, 3414426687606941972, 18161196869091297655], absorbed := 3 }
+  , cursorAfter := { stateWords := [11236326198904743827, 14532122700454992670, 10802315202157041540, 13369252553900132433, 5234822617317489414, 525355939062290597, 18087254811635658711, 3351311869823913135], absorbed := 0 }
+  , challengeOutput := (some 11236326198904743827)
   , digestOutput := none
 }, {
   kind := .appendMessage
   , label := (bytes [114, 118, 54, 52, 105, 109, 47, 107, 101, 114, 110, 101, 108, 47, 115, 116, 97, 103, 101, 51, 95, 100, 105, 103, 101, 115, 116])
   , message := (bytes [242, 180, 211, 44, 136, 191, 129, 103, 121, 27, 189, 177, 57, 84, 107, 37, 200, 205, 250, 244, 70, 251, 148, 129, 186, 236, 174, 139, 158, 109, 21, 76])
   , u64s := []
-  , cursorBefore := { stateWords := [18307016013854385768, 386090934767535184, 301195876403596823, 8691723873807917873, 16010316393357224490, 5609107225314861888, 2143909010010563256, 617300435659316442], absorbed := 0 }
-  , cursorAfter := { stateWords := [19972606401193323, 39317353527350523, 1276472734, 16900528731064752535, 15933562643972886562, 9693504331108410883, 18331968259489044684, 11793688974313911503], absorbed := 3 }
+  , cursorBefore := { stateWords := [11236326198904743827, 14532122700454992670, 10802315202157041540, 13369252553900132433, 5234822617317489414, 525355939062290597, 18087254811635658711, 3351311869823913135], absorbed := 0 }
+  , cursorAfter := { stateWords := [19972606401193323, 39317353527350523, 1276472734, 16274229555519422653, 16974672749192474638, 4430053409062725850, 16438097491389033793, 15433633138756558878], absorbed := 3 }
   , challengeOutput := none
   , digestOutput := none
 }, {
   kind := .appendMessage
   , label := (bytes [114, 118, 54, 52, 105, 109, 47, 107, 101, 114, 110, 101, 108, 47, 101, 120, 101, 99, 117, 116, 105, 111, 110, 95, 100, 105, 103, 101, 115, 116])
-  , message := (bytes [45, 139, 239, 85, 27, 12, 138, 44, 207, 170, 242, 243, 57, 214, 167, 103, 64, 10, 131, 45, 76, 123, 145, 234, 211, 58, 109, 152, 0, 38, 77, 105])
+  , message := (bytes [48, 44, 208, 21, 233, 188, 246, 118, 80, 252, 131, 40, 26, 233, 88, 199, 128, 90, 68, 220, 142, 222, 119, 79, 4, 89, 207, 71, 146, 168, 93, 57])
   , u64s := []
-  , cursorBefore := { stateWords := [19972606401193323, 39317353527350523, 1276472734, 16900528731064752535, 15933562643972886562, 9693504331108410883, 18331968259489044684, 11793688974313911503], absorbed := 3 }
-  , cursorAfter := { stateWords := [21442139065968551, 42904295890915707, 1766663680, 10458115475421553961, 9773600212131026291, 13845302979605083383, 9838001921692512024, 15293084120696307460], absorbed := 3 }
+  , cursorBefore := { stateWords := [19972606401193323, 39317353527350523, 1276472734, 16274229555519422653, 16974672749192474638, 4430053409062725850, 16438097491389033793, 15433633138756558878], absorbed := 3 }
+  , cursorAfter := { stateWords := [40211632827189080, 20212704577812446, 962439314, 6039256894354310933, 6031758554601834355, 11278688584296007858, 3893914303756742345, 4253956639539515579], absorbed := 3 }
   , challengeOutput := none
   , digestOutput := none
 }, {
@@ -240,8 +276,8 @@ def derivedCase : ParityDerivedCase :=
   , label := (bytes [114, 118, 54, 52, 105, 109, 47, 107, 101, 114, 110, 101, 108, 47, 102, 105, 110, 97, 108, 95, 115, 116, 97, 116, 101, 95, 100, 105, 103, 101, 115, 116])
   , message := (bytes [241, 21, 138, 101, 163, 40, 99, 15, 168, 152, 12, 213, 123, 114, 205, 136, 161, 172, 16, 50, 10, 193, 235, 221, 241, 226, 242, 67, 57, 144, 122, 37])
   , u64s := []
-  , cursorBefore := { stateWords := [21442139065968551, 42904295890915707, 1766663680, 10458115475421553961, 9773600212131026291, 13845302979605083383, 9838001921692512024, 15293084120696307460], absorbed := 3 }
-  , cursorAfter := { stateWords := [2869796964239565, 19125879973997505, 628789305, 1917667635319776294, 9398324432138629513, 18287976505901795566, 578311037544406826, 10417819720721837766], absorbed := 3 }
+  , cursorBefore := { stateWords := [40211632827189080, 20212704577812446, 962439314, 6039256894354310933, 6031758554601834355, 11278688584296007858, 3893914303756742345, 4253956639539515579], absorbed := 3 }
+  , cursorAfter := { stateWords := [2869796964239565, 19125879973997505, 628789305, 15867107718016502534, 742118945884326825, 3231925605746862542, 9406865583467843754, 7361031662932662875], absorbed := 3 }
   , challengeOutput := none
   , digestOutput := none
 }, {
@@ -249,34 +285,34 @@ def derivedCase : ParityDerivedCase :=
   , label := (bytes [114, 118, 54, 52, 105, 109, 47, 107, 101, 114, 110, 101, 108, 47, 102, 105, 110, 97, 108, 95, 109, 105, 120])
   , message := (bytes [])
   , u64s := []
-  , cursorBefore := { stateWords := [2869796964239565, 19125879973997505, 628789305, 1917667635319776294, 9398324432138629513, 18287976505901795566, 578311037544406826, 10417819720721837766], absorbed := 3 }
-  , cursorAfter := { stateWords := [10198769342489062892, 9560620643758735775, 883114345830561381, 1543446596572376349, 927444997298294527, 2093159359449483533, 5723733942285223712, 5465858754595007560], absorbed := 0 }
-  , challengeOutput := (some 10198769342489062892)
+  , cursorBefore := { stateWords := [2869796964239565, 19125879973997505, 628789305, 15867107718016502534, 742118945884326825, 3231925605746862542, 9406865583467843754, 7361031662932662875], absorbed := 3 }
+  , cursorAfter := { stateWords := [9465929736532604617, 8420220252723389205, 3417381235763225621, 4183586137376879782, 5900319465490910417, 9092472782636357916, 17349179717391889123, 17539475516024234292], absorbed := 0 }
+  , challengeOutput := (some 9465929736532604617)
   , digestOutput := none
 }, {
   kind := .digest32
   , label := (bytes [])
   , message := (bytes [])
   , u64s := []
-  , cursorBefore := { stateWords := [10198769342489062892, 9560620643758735775, 883114345830561381, 1543446596572376349, 927444997298294527, 2093159359449483533, 5723733942285223712, 5465858754595007560], absorbed := 0 }
-  , cursorAfter := { stateWords := [15419860829055723611, 2987260217215641730, 9435454222050012773, 6365062609455462017, 11259537094546917016, 7651890499768272024, 10334182728623754604, 9408803761618098517], absorbed := 0 }
+  , cursorBefore := { stateWords := [9465929736532604617, 8420220252723389205, 3417381235763225621, 4183586137376879782, 5900319465490910417, 9092472782636357916, 17349179717391889123, 17539475516024234292], absorbed := 0 }
+  , cursorAfter := { stateWords := [4389844868881287918, 16069944125868069814, 18074736236063466078, 270298057294202076, 5337330470334798401, 7728982227267766060, 2381843619493432972, 12046089070115929937], absorbed := 0 }
   , challengeOutput := none
-  , digestOutput := (some (bytes [91, 168, 211, 225, 185, 89, 254, 213, 130, 104, 203, 34, 87, 225, 116, 41, 101, 46, 192, 175, 159, 119, 241, 130, 129, 182, 182, 65, 184, 62, 85, 88]))
+  , digestOutput := (some (bytes [238, 138, 189, 92, 166, 220, 235, 60, 182, 211, 189, 78, 10, 233, 3, 223, 94, 162, 113, 183, 215, 92, 214, 250, 220, 196, 127, 168, 166, 74, 192, 3]))
 }]
 }
   , kernel := {
   root0Digest := (bytes [196, 47, 73, 21, 89, 47, 90, 96, 97, 14, 113, 80, 57, 244, 48, 50, 219, 255, 79, 205, 86, 212, 1, 182, 140, 236, 129, 158, 228, 112, 219, 0])
-  , stage1Digest := (bytes [133, 33, 172, 140, 233, 72, 46, 209, 48, 165, 182, 74, 209, 48, 22, 152, 88, 9, 98, 197, 159, 186, 241, 163, 39, 42, 69, 121, 8, 165, 34, 71])
-  , stage2Digest := (bytes [99, 28, 72, 198, 124, 237, 213, 46, 85, 239, 4, 76, 205, 104, 112, 135, 151, 48, 199, 18, 8, 29, 82, 0, 29, 46, 209, 175, 11, 65, 240, 59])
+  , stage1Digest := (bytes [142, 217, 182, 138, 150, 76, 176, 209, 117, 25, 246, 139, 222, 66, 241, 101, 236, 89, 218, 142, 67, 238, 206, 4, 53, 48, 117, 115, 130, 138, 60, 69])
+  , stage2Digest := (bytes [227, 21, 223, 164, 30, 253, 30, 252, 35, 185, 19, 78, 208, 4, 88, 134, 20, 175, 97, 180, 193, 112, 119, 234, 96, 78, 211, 206, 96, 42, 169, 244])
   , stage3Digest := (bytes [242, 180, 211, 44, 136, 191, 129, 103, 121, 27, 189, 177, 57, 84, 107, 37, 200, 205, 250, 244, 70, 251, 148, 129, 186, 236, 174, 139, 158, 109, 21, 76])
-  , executionDigest := (bytes [45, 139, 239, 85, 27, 12, 138, 44, 207, 170, 242, 243, 57, 214, 167, 103, 64, 10, 131, 45, 76, 123, 145, 234, 211, 58, 109, 152, 0, 38, 77, 105])
+  , executionDigest := (bytes [48, 44, 208, 21, 233, 188, 246, 118, 80, 252, 131, 40, 26, 233, 88, 199, 128, 90, 68, 220, 142, 222, 119, 79, 4, 89, 207, 71, 146, 168, 93, 57])
   , finalStateDigest := (bytes [241, 21, 138, 101, 163, 40, 99, 15, 168, 152, 12, 213, 123, 114, 205, 136, 161, 172, 16, 50, 10, 193, 235, 221, 241, 226, 242, 67, 57, 144, 122, 37])
   , stage1Mix := 1056787187556541480
-  , stage2RegMix := 4238065095073052119
-  , stage2RamMix := 14880338601956528058
-  , stage3ContinuityMix := 18307016013854385768
-  , kernelFinalMix := 10198769342489062892
-  , transcriptFinalDigest := (bytes [91, 168, 211, 225, 185, 89, 254, 213, 130, 104, 203, 34, 87, 225, 116, 41, 101, 46, 192, 175, 159, 119, 241, 130, 129, 182, 182, 65, 184, 62, 85, 88])
+  , stage2RegMix := 9619277481828672587
+  , stage2RamMix := 16812727767669355212
+  , stage3ContinuityMix := 11236326198904743827
+  , kernelFinalMix := 9465929736532604617
+  , transcriptFinalDigest := (bytes [238, 138, 189, 92, 166, 220, 235, 60, 182, 211, 189, 78, 10, 233, 3, 223, 94, 162, 113, 183, 215, 92, 214, 250, 220, 196, 127, 168, 166, 74, 192, 3])
   , finalPc := 16
   , finalRegisters := [0, 42, 42, 0, 0, 0, 0, 0, 0, 0, 8200, 0, 0, 0, 0, 0, 0, 0, 0, 0, 0, 0, 0, 0, 0, 0, 0, 0, 0, 0, 0, 0]
   , finalMemory := [{ addr := 8192, value := 42 }, { addr := 8200, value := 99 }]
